lemmasTotorial.dfy
@@ -1,0 +1,58 @@
+//Searching for Zero
+lemma SkippingLemma(a : array?<int>, j : int)
+   requires a != null
+   requires forall i :: 0 <= i < a.Length ==> 0 <= a[i]
+   requires forall i :: 0 < i < a.Length ==> a[i-1]-1 <= a[i]
+   requires 0 <= j < a.Length
+   ensures forall i :: j <= i < j + a[j] && i < a.Length ==> a[i] != 0
+{
+   var i := j;
+   while i < j + a[j] && i < a.Length
+      decreases j + a[j] - i
+      invariant i < a.Length ==> a[j] - (i-j) <= a[i]
+      invariant forall k :: j <= k < i && k < a.Length ==> a[k] != 0
+   {
+      i := i + 1;
+   }
+}
+method FindZero(a: array?<int>) returns (index: int)
+   requires a != null
+   requires forall i :: 0 <= i < a.Length ==> 0 <= a[i]
+   requires forall i :: 0 < i < a.Length ==> a[i-1]-1 <= a[i]
+   ensures index < 0  ==> forall i :: 0 <= i < a.Length ==> a[i] != 0
+   ensures 0 <= index ==> index < a.Length && a[index] == 0
+{
+   index := 0;
+   while index < a.Length
+      decreases a.Length - index
+      invariant 0 <= index
+      invariant forall k :: 0 <= k < index && k < a.Length ==> a[k] != 0
+   {
+      if a[index] == 0 { return; }
+      SkippingLemma(a, index);
+      index := index + a[index];
+   }
+   index := -1;
+}
+
+//Counting
+lemma DistributiveLemma(a: seq<bool>, b: seq<bool>)
+   decreases a, b
+   ensures count(a + b) == count(a) + count(b)
+{
+   if a == []
+   {
+      assert a + b == b;
+   }
+   else
+   {
+      DistributiveLemma(a[1..], b);
+      assert a + b == [a[0]] + (a[1..] + b);
+   }
+}
+function count(a: seq<bool>): nat
+   decreases a
+{
+   if |a| == 0 then 0 else
+   (if a[0] then 1 else 0) + count(a[1..])
+}
